Veritas.MultiSetHash.fsti
@@ -43,21 +43,18 @@ type ms_hashfn_dom =
 val ms_hashfn_upd (e: ms_hashfn_dom) (h: ms_hash_value): Tot ms_hash_value
 
 (* multiset hash function for a sequence *)
-let rec ms_hashfn (s: seq ms_hashfn_dom): Tot ms_hash_value 
-  (decreases (length s)) = 
-  let n = length s in
-  (* empty sequence *)
-  if n = 0 then empty_hash_value
-  else
-    let s' = prefix s (n - 1) in
-    let e' = index s (n - 1) in
-    let h' = ms_hashfn s' in
-    ms_hashfn_upd e' h'
+val ms_hashfn (s: seq ms_hashfn_dom): Tot ms_hash_value 
 
 (* two sequences that encode the same multiset produce the same hash *)
 val lemma_mshashfn_correct (s1 s2: seq ms_hashfn_dom):
   Lemma (requires (seq2mset s1 == seq2mset s2))
         (ensures (ms_hashfn s1 = ms_hashfn s2))
+
+(* aggregation of multiset hashes *)
+val ms_hashfn_agg (h1: ms_hash_value) (h2: ms_hash_value) : Tot ms_hash_value
+
+val lemma_hashfn_agg (s1 s2: seq ms_hashfn_dom):
+  Lemma (ms_hashfn (append s1 s2) = ms_hashfn_agg (ms_hashfn s1) (ms_hashfn s2))
 
 (* multiset hash collision *)
 type ms_hash_collision = 
