Veritas.MultiSetHash.fst
@@ -1,0 +1,32 @@
+module Veritas.MultiSetHash
+
+(* Hash value of an empty set *)
+let empty_hash_value: ms_hash_value = zero_vec 
+
+let ms_hashfn_upd (e: ms_hashfn_dom) (h: ms_hash_value): Tot ms_hash_value = admit()
+
+(* multiset hash function for a sequence *)
+let rec ms_hashfn_aux (s: seq ms_hashfn_dom): Tot ms_hash_value 
+  (decreases (length s)) = 
+  let n = length s in
+  (* empty sequence *)
+  if n = 0 then empty_hash_value
+  else
+    let s' = prefix s (n - 1) in
+    let e' = index s (n - 1) in
+    let h' = ms_hashfn_aux s' in
+    ms_hashfn_upd e' h'
+
+(* multiset hash function for a sequence *)
+let ms_hashfn (s: seq ms_hashfn_dom): Tot ms_hash_value = ms_hashfn_aux s
+
+(* two sequences that encode the same multiset produce the same hash *)
+let lemma_mshashfn_correct (s1 s2: seq ms_hashfn_dom):
+  Lemma (requires (seq2mset s1 == seq2mset s2))
+        (ensures (ms_hashfn s1 = ms_hashfn s2)) = admit()
+
+(* aggregation of multiset hashes *)
+let ms_hashfn_agg (h1: ms_hash_value) (h2: ms_hash_value) : Tot ms_hash_value = admit()
+
+let lemma_hashfn_agg (s1 s2: seq ms_hashfn_dom):
+  Lemma (ms_hashfn (append s1 s2) = ms_hashfn_agg (ms_hashfn s1) (ms_hashfn s2)) = admit()
