Makefile
@@ -12,7 +12,7 @@ FSTAR_FILES := Veritas.BinTree.fsti Veritas.BinTree.fst \
                Veritas.Key.fsti Veritas.Record.fsti \
                Veritas.SeqAux.fsti Veritas.SeqAux.fst \
                Veritas.MultiSet.fsti Veritas.MultiSet.fst \
-               Veritas.MultiSetHash.fsti \
+               Veritas.MultiSetHash.fsti Veritas.MultiSetHash.fst \
                Veritas.Hash.fsti \
                Veritas.SeqOps.fsti Veritas.SeqOps.fst \
                Veritas.Verifier.fst \
